rocq/Compile.mli
@@ -9,7 +9,21 @@ val aop_instr : aop -> reg -> reg -> instr
 
 val gen_var : var -> reg -> code
 
+val is_flag_expr : expr -> bool
+
+val is_nz_test : binop -> expr -> bool
+
+val nz_code : (reg -> code) -> (reg -> code) -> reg -> code
+
+val flag_code : bool -> (reg -> code) -> (reg -> code) -> reg -> code
+
+val unflag_code : bool -> (reg -> code) -> (reg -> code) -> reg -> code
+
+val cmp_fwd : binop -> reg -> reg -> reg -> reg -> code
+
 val gen_expr : expr -> reg -> code
+
+val ungen_expr : expr -> reg -> code
 
 val gen_assign : var -> aop -> expr -> code
 
