rocq/PISA.mli
@@ -22,6 +22,8 @@ type instr =
 | INeg of reg
 | IExch of reg * reg
 | ISltx of reg * reg * reg
+| IOrx of reg * reg
+| IAndx of reg * reg * reg
 
 type code = instr list
 
