rocq/PosDef.mli
@@ -22,6 +22,12 @@ module Pos :
 
   val coq_Ndouble : int -> int
 
+  val coq_lor : int -> int -> int
+
+  val coq_land : int -> int -> int
+
+  val ldiff : int -> int -> int
+
   val coq_lxor : int -> int -> int
 
   val of_succ_nat : int -> int
